more

Weidenbach_Book/CDCL_Two_Watched_Literals_List_Simple_Code.thy
@@ -29,23 +29,333 @@ definition backtrack_list' :: "'v twl_st_list \<Rightarrow> 'v twl_st_list nres"
     }
   \<close>
 
-lemma
+lemma Let_assignI: \<open>\<Phi> = {L'} \<Longrightarrow> P L' = Q L' \<Longrightarrow>  (do {let L = L'; P L}) = (do {L \<leftarrow> RES \<Phi>; Q L})\<close>
+  by (simp add: RES_sng_eq_RETURN)
+
+lemma bt_cut_not_none2:
+  assumes "no_dup M"  and "i < count_decided M"
+  shows "bt_cut i M \<noteq> None"
+proof -
+  obtain K M1 M2 where 
+    \<open>M = M2 @ Decided K # M1\<close> and \<open>get_level M K = Suc i\<close>
+      using le_count_decided_decomp[OF assms(1)] assms(2) by auto
+    then show ?thesis
+      using bt_cut_not_none[OF assms(1), of M2 K M1 i] by auto
+qed
+
+lemma backtrack_list'_spec:
   assumes
-    \<open>get_conflict_list S \<noteq> None \<and> get_conflict_list S \<noteq> Some [] \<and>
-       working_queue_list S = {#} \<and> pending_list S = {#} \<and> additional_WS_invs S \<and>
-       no_step cdcl\<^sub>W_restart_mset.skip (convert_to_state (twl_st_of S)) \<and>
-       no_step cdcl\<^sub>W_restart_mset.resolve (convert_to_state (twl_st_of S)) \<and>
-       twl_struct_invs (twl_st_of S) \<and> twl_stgy_invs (twl_st_of S)\<close>
-  shows \<open>(backtrack_list', backtrack_list) \<in> 
-    {(S', S). S' = S \<and> get_conflict_list S \<noteq> None \<and> get_conflict_list S \<noteq> Some [] \<and>
-       working_queue_list S = {#} \<and> pending_list S = {#} \<and> additional_WS_invs S \<and>
-       no_step cdcl\<^sub>W_restart_mset.skip (convert_to_state (twl_st_of S)) \<and>
-       no_step cdcl\<^sub>W_restart_mset.resolve (convert_to_state (twl_st_of S)) \<and>
-       twl_struct_invs (twl_st_of S) \<and> twl_stgy_invs (twl_st_of S)} \<rightarrow> {(S', S). S' = S}\<close>
-  unfolding backtrack_list_def backtrack_list'_def
+    confl1: \<open>get_conflict_list S \<noteq> None\<close> and
+    confl2: \<open>get_conflict_list S \<noteq> Some []\<close> and
+    \<open>working_queue_list S = {#}\<close> and
+    \<open>pending_list S = {#}\<close> and
+    \<open>additional_WS_invs S\<close> and
+    ns: \<open>no_step cdcl\<^sub>W_restart_mset.skip (convert_to_state (twl_st_of S))\<close> and
+    \<open>no_step cdcl\<^sub>W_restart_mset.resolve (convert_to_state (twl_st_of S))\<close> and
+    struct_invs: \<open>twl_struct_invs (twl_st_of S)\<close> and
+    stgy_invs: \<open>twl_stgy_invs (twl_st_of S)\<close> (* and
+    SS: \<open>S' = S\<close> *)
+  shows \<open>backtrack_list' S \<le> \<Down> Id (backtrack_list S)\<close>
+proof- 
+  show ?thesis
+    unfolding backtrack_list_def backtrack_list'_def (* SS *)
     apply (rewrite at \<open>let _ = snd _ in _\<close> Let_def)
-  apply refine_rcg
-  apply (case_tac a')
-  apply (refine_vcg ASSERT_same_eq_conv[THEN iffD2])
-sorry
+    apply (refine_rcg; remove_dummy_vars)
+    subgoal by simp
+    subgoal by simp
+    subgoal by simp
+    subgoal by simp
+    subgoal premises p for M N U C NP UP WS Q L
+    proof -  
+      note S = p(1) and L = p(4) and M_not_empty = p(2) and ex_decomp = p(8)
+      have n_d: \<open>no_dup M\<close>
+        using struct_invs unfolding twl_struct_invs_def cdcl\<^sub>W_restart_mset.cdcl\<^sub>W_all_struct_inv_def cdcl\<^sub>W_restart_mset.cdcl\<^sub>W_M_level_inv_def
+        by (simp add: cdcl\<^sub>W_restart_mset_state S)
+      obtain C' where [simp]: \<open>C = Some C'\<close>
+        using confl1 S by auto
+      have lev_L: \<open>get_level M L = count_decided M\<close>
+        using M_not_empty L by (cases M) auto
+      have uhd_C: \<open>- lit_of (hd (convert_lits_l N M)) \<in> set C'\<close>
+        using cdcl\<^sub>W_restart_mset.no_step_skip_hd_in_conflicting[of
+            \<open>convert_to_state (twl_st_of (M, N, U, C, NP, UP, WS, Q))\<close>]
+        confl2 ns struct_invs stgy_invs unfolding S
+        by (auto simp: twl_struct_invs_def twl_stgy_invs_def cdcl\<^sub>W_restart_mset_state)
+      obtain M1'' M2'' K'' where
+        decomp_K'': \<open>(Decided K'' # M1'', M2'') \<in> set (get_all_ann_decomposition M)\<close>
+        \<open>get_level M K'' = Suc (get_maximum_level M (remove1_mset (- lit_of (hd M)) (mset C')))\<close>
+        using ex_decomp by auto
+      then have lev_max: \<open>get_maximum_level M (mset (remove1 (-L) C')) < count_decided M\<close>
+        using count_decided_ge_get_level[of M K''] L by auto
+      have \<open>-L \<in># mset C'\<close>
+        using uhd_C L M_not_empty by (cases M) simp_all
+      with multi_member_split[OF this]
+      have False if \<open>find_level_decomp M (the C) [] (count_decided M) = None\<close>
+        using find_level_decomp_none[OF that, of \<open>-L\<close> \<open>remove1 (-L) C'\<close>] lev_max
+        unfolding S by (auto dest!: simp: lev_L)
+      then obtain K j where
+        Kj: \<open>find_level_decomp M C' [] (count_decided M) = Some (K, j)\<close>
+        by (cases \<open>find_level_decomp M (the C) [] (count_decided M)\<close>) auto
+      then have 
+        \<open>K \<in> set C'\<close> and
+        j: \<open>get_maximum_level M (mset (remove1 K C')) = j\<close> and
+        \<open>get_level M K = count_decided M\<close>
+        using find_level_decomp_some[OF Kj] by simp_all
+      have KL: \<open>K = -L\<close>
+        by (metis \<open>K \<in> set C'\<close> \<open>\<exists>A. mset C' = add_mset (- L) A\<close> \<open>get_level M K = count_decided M\<close> 
+            add_mset_remove_trivial get_maximum_level_ge_get_level leD lev_max member_add_mset
+            mset_remove1 set_mset_mset)
+      have j_le_M: \<open>j < count_decided M\<close>
+          unfolding j[symmetric] KL using lev_max by simp
+      have \<open>bt_cut j M \<noteq> None\<close>
+        apply (rule bt_cut_not_none2[of ])
+        using n_d apply (simp; fail)
+        using j_le_M by simp
+      then obtain M2 M1 K''' M' where
+        \<open>M = M2 @ M'\<close> and M': \<open>M' = Decided K''' # M1\<close> and lev_K: \<open>get_level M K''' = j + 1\<close> and
+        bt_cut: \<open>bt_cut j M = Some M'\<close>
+        using bt_cut_some_decomp[of M j \<open>the (bt_cut j M)\<close>] n_d by auto
+      show ?thesis
+        using lev_K j bt_cut_in_get_all_ann_decomposition[OF n_d bt_cut] by (auto simp: Kj bt_cut M' KL)
+    qed
+    subgoal premises p for M N U C NP UP WS Q L M1
+    proof -
+      note S = p(1) and L_hd = p(4) and len_C = p(11)
+      obtain C' where [simp]: \<open>C = Some C'\<close>
+        using confl1 S by auto
+      
+      have \<open>find (\<lambda>L'. get_level M L' = get_maximum_level M (remove1_mset (- L) (mset (the C)))) (the C) \<noteq> None\<close>
+      proof (rule ccontr)
+        assume H: \<open>\<not>?thesis\<close>
+        have \<open>remove1_mset (- lit_of (hd M)) (mset (the C)) \<noteq> {#}\<close>
+          using len_C by (cases C'; cases \<open>tl C'\<close>) (auto simp: Diff_eq_empty_iff_mset)
+        then show False
+          using get_maximum_level_exists_lit_of_max_level[of 
+              \<open>remove1_mset (- lit_of (hd M)) (mset (the C))\<close> M]
+          using L_hd H by (auto simp: find_None_iff dest: in_diffD)
+      qed
+      then show ?thesis
+        using p by (auto dest: find_SomeD)
+    qed
+    subgoal by simp
+    subgoal by simp
+    done
+qed
+
+definition cdcl_twl_o_prog_list' :: "'v twl_st_list \<Rightarrow> (bool \<times> 'v twl_st_list) nres"  where
+  \<open>cdcl_twl_o_prog_list' S =
+    do {
+      let (M, N, U, D, NP, UP, WS, Q) = S in
+      do {
+        if D = None
+        then
+          if (\<exists>L. undefined_lit M L \<and> atm_of L \<in> atms_of_mm (clause `# twl_clause_of `# mset (take U (tl N))))
+          then do {S \<leftarrow> decide_list S; RETURN (False, S)}
+          else do {RETURN (True, S)}
+        else do {
+          T \<leftarrow> skip_and_resolve_loop_list S;
+          if get_conflict_list T \<noteq> Some []
+          then do {U \<leftarrow> backtrack_list' T; RETURN (False, U)}
+          else do {RETURN (True, T)}
+        }
+      }
+    }
+  \<close>
+
+lemma TT:
+  assumes \<open>(f, g) \<in> {(S, S'). S' = h S \<and> P S} \<rightarrow> \<langle>{(T, T'). T' = h' T \<and> Q T}\<rangle>nres_rel\<close> and 
+    \<open>P S\<close> and \<open>\<And>S. P S \<Longrightarrow> nofail (g (h S))\<close>
+  shows \<open>f S \<le> \<Down> {(T', T). T = T' \<and> Q T} (f S)\<close>
+  using assms unfolding fun_rel_def nres_rel_def 
+  by (auto simp add: pw_conc_inres pw_conc_nofail pw_ords_iff(1))
+
+lemma TT':
+  assumes \<open>f \<le> \<Down> R g\<close> and \<open>g \<le> \<Down> R' h\<close>
+  shows \<open>f \<le> \<Down> (R O R') h\<close>
+  by (metis (full_types) assms(1) assms(2) conc_fun_chain ref_two_step)
+
+thm TT'[OF backtrack_list'_spec backtrack_list_spec[THEN refine_pair_to_SPEC]]
+
+lemma cdcl_twl_o_prog_list_spec:
+  \<open>(cdcl_twl_o_prog_list', cdcl_twl_o_prog) \<in>
+    {(S, S'). S' = twl_st_of S \<and>
+       working_queue_list S = {#} \<and> pending_list S = {#} \<and> no_step cdcl_twl_cp (twl_st_of S) \<and>
+       twl_struct_invs (twl_st_of S) \<and> twl_stgy_invs (twl_st_of S) \<and> additional_WS_invs S} \<rightarrow>
+    \<langle>{((brk, T), (brk', T')). T' = twl_st_of T \<and> brk = brk' \<and> additional_WS_invs T \<and>
+    (get_conflict_list T \<noteq> None \<longrightarrow> get_conflict_list T = Some [])\<and>
+       twl_struct_invs (twl_st_of T) \<and> twl_stgy_invs (twl_st_of T) \<and> working_queue_list T = {#} (* \<and>
+       (\<not>brk \<longrightarrow> pending_list T \<noteq> {#}) *)}\<rangle> nres_rel\<close>
+  (is \<open> _ \<in> ?R \<rightarrow> ?I\<close> is \<open> _ \<in> ?R \<rightarrow> \<langle>?J\<rangle>nres_rel\<close>)
+proof -
+  have twl_prog:
+    \<open>(cdcl_twl_o_prog_list', cdcl_twl_o_prog) \<in> ?R \<rightarrow>
+      \<langle>{(S, S').
+         (fst S' = (fst S) \<and> snd S' = twl_st_of (snd S)) \<and> additional_WS_invs (snd S)}\<rangle> nres_rel\<close>
+    apply clarify
+    unfolding cdcl_twl_o_prog_list'_def cdcl_twl_o_prog_def
+    apply (refine_vcg decide_list_spec[THEN refine_pair_to_SPEC]
+        skip_and_resolve_loop_list_spec[THEN refine_pair_to_SPEC]
+        TT'[OF backtrack_list'_spec backtrack_list_spec[THEN refine_pair_to_SPEC]];
+        remove_dummy_vars)
+    subgoal by simp
+    subgoal by simp
+    subgoal for M N U NP UP WS Q M' N' U' NP' UP' WS' Q'
+      by (simp add: additional_WS_invs_def)
+    subgoal for M N U NP UP WS Q M' N' U' NP' UP' WS' Q'
+      by simp
+    subgoal for M N U NP UP WS Q M' N' U' NP' UP' WS' Q'
+      by simp
+    subgoal for M N U NP UP WS Q M' N' U' NP' UP' WS' Q'
+      by (simp add: additional_WS_invs_def)
+    subgoal for M N U NP UP WS Q M' N' U' NP' UP' WS' Q'
+      by auto
+    subgoal for M N U NP UP WS Q M' N' U' NP' UP' WS' Q' _ _ T
+      by (cases T) (auto)
+    subgoal for M N U NP UP WS Q M' N' U' NP' UP' WS' Q' _ _ T
+      apply (cases M; cases T)
+      by (auto simp add: additional_WS_invs_def)
+    subgoal for M N U NP UP WS Q M' N' U' NP' UP' WS' Q'
+      by auto
+    subgoal for M N U NP UP WS Q M' N' U' NP' UP' WS' Q' _ _ T
+      by (cases T) (auto)
+    subgoal for M N U NP UP WS Q M' N' U' NP' UP' WS' Q' _ _ T
+      by (auto simp add: get_conflict_list_Some_nil_iff)
+    subgoal for M N U NP UP WS Q M' N' U' NP' UP' WS' Q' _ _ T
+      by fast
+    subgoal for M N U NP UP WS Q M' N' U' NP' UP' WS' Q'
+      by fast
+    subgoal for M N U NP UP WS Q M' N' U' NP' UP' WS' Q' _ _ T
+      by (cases T) (auto)
+    subgoal for M N U NP UP WS Q M' N' U' NP' UP' WS' Q' _ _ T T'
+      by fast
+    subgoal for M N U NP UP WS Q M' N' U' NP' UP' WS' Q'
+      by (simp add: get_conflict_list_get_conflict)
+    subgoal for M N U NP UP WS Q M' N' U' NP' UP' WS' Q' _ _ T
+      apply (cases M; cases T)
+      by (auto simp add: additional_WS_invs_def)
+    subgoal for M N U NP UP WS Q M' N' U' NP' UP' WS' Q' _ _ T
+      apply (cases M; cases T)
+      by (auto simp add: (* additional_WS_invs_def *))
+    subgoal by fast
+    subgoal by fast
+    subgoal by fast
+    subgoal by fast
+    subgoal by fast
+    subgoal by fast
+    subgoal by simp
+    subgoal by simp
+    done
+  have KK:
+    \<open>get_conflict_list T = None \<longleftrightarrow> get_conflict (twl_st_of T) = None\<close>
+    \<open>working_queue_list T = {#} \<longleftrightarrow> working_queue (twl_st_of T) = {#}\<close>
+    \<open>pending_list T = {#} \<longleftrightarrow> pending (twl_st_of T) = {#}\<close>
+    for T
+    by (cases T; auto)+
+  text \<open>Stupid placeholder to help the application of \<open>rule\<close> later:\<close>
+  define TT where [simp]: \<open>TT = (\<lambda>_::bool \<times> 'a twl_st_list. True)\<close>
+  let ?J' = \<open>{(U, U').
+       (fst U' = id (fst U) \<and> snd U' = twl_st_of (snd U)) \<and> additional_WS_invs (snd U) \<and>
+        (get_conflict (twl_st_of (snd U)) \<noteq> None \<longrightarrow> get_conflict (twl_st_of (snd U)) = Some {#}) \<and>
+         twl_struct_invs (twl_st_of (snd U)) \<and>
+         twl_stgy_invs (twl_st_of (snd U)) \<and>
+         working_queue (twl_st_of (snd U)) = {#} (* \<and>
+         (\<not>fst U \<longrightarrow> pending (twl_st_of (snd U)) \<noteq> {#}) *)}\<close>
+
+  have J: \<open>?J = ?J'\<close>
+    by auto
+  show bt': ?thesis
+    unfolding J
+    apply (rule refine_add_inv_pair)
+    subgoal
+      using twl_prog by (auto simp:)
+    subgoal for S
+      apply (rule weaken_SPEC[OF cdcl_twl_o_prog_spec[of \<open>twl_st_of S\<close>]])
+      apply (auto simp: KK(3))[5]
+      apply auto
+      done
+    done
+qed
+
+
+definition cdcl_twl_stgy_prog_list' :: "'v twl_st_list \<Rightarrow> 'v twl_st_list nres"  where
+  \<open>cdcl_twl_stgy_prog_list' S\<^sub>0 =
+  do {
+    do {
+      (brk, T) \<leftarrow> WHILE\<^sub>T\<^bsup>\<lambda>(brk, T). twl_struct_invs (twl_st_of T) \<and> twl_stgy_invs (twl_st_of T) \<and>
+        (brk \<longrightarrow> no_step cdcl_twl_stgy (twl_st_of T)) \<and> cdcl_twl_stgy\<^sup>*\<^sup>* (twl_st_of S\<^sub>0) (twl_st_of T) \<and>
+        working_queue_list T = {#} \<and>
+        (\<not>brk \<longrightarrow> get_conflict_list T = None)\<^esup>
+        (\<lambda>(brk, _). \<not>brk)
+        (\<lambda>(brk, S).
+        do {
+          T \<leftarrow> unit_propagation_outer_loop_list S;
+          cdcl_twl_o_prog_list' T
+        })
+        (False, S\<^sub>0);
+      RETURN T
+    }
+  }
+  \<close>
+
+
+lemma cdcl_twl_stgy_prog_list'_spec:
+  \<open>(cdcl_twl_stgy_prog_list', cdcl_twl_stgy_prog) \<in>
+    {(S, S'). S' = twl_st_of S \<and> additional_WS_invs S \<and>
+       working_queue_list S = {#} \<and>
+       twl_struct_invs (twl_st_of S) \<and> twl_stgy_invs (twl_st_of S)} \<rightarrow>
+    \<langle>{(T, T'). T' = twl_st_of T \<and> True}\<rangle> nres_rel\<close>
+  (is \<open> _ \<in> ?R \<rightarrow> ?I\<close> is \<open> _ \<in> ?R \<rightarrow> \<langle>?J\<rangle>nres_rel\<close>)
+proof -
+  have R: \<open>(a, b) \<in> ?R \<Longrightarrow> ((False, a), (False, b)) \<in> {((brk, S), (brk', S')). brk = brk' \<and> (S, S') \<in> ?R}\<close>
+    for a b by auto
+  have KK:
+    \<open>get_conflict_list T = None \<longleftrightarrow> get_conflict (twl_st_of T) = None\<close>
+    \<open>working_queue_list T = {#} \<longleftrightarrow> working_queue (twl_st_of T) = {#}\<close>
+    \<open>pending_list T = {#} \<longleftrightarrow> pending (twl_st_of T) = {#}\<close>
+    for T
+    by (cases T; auto)+
+  show ?thesis
+    unfolding cdcl_twl_stgy_prog_list'_def cdcl_twl_stgy_prog_def
+    apply (refine_rcg R cdcl_twl_o_prog_list_spec[THEN refine_pair_to_SPEC2]
+        unit_propagation_outer_loop_list_spec[THEN refine_pair_to_SPEC]; remove_dummy_vars)
+    subgoal unfolding KK by auto
+    subgoal by auto
+    subgoal by fastforce
+    subgoal unfolding KK by fastforce
+    subgoal by auto
+    subgoal unfolding KK by auto
+    subgoal unfolding KK by auto
+    subgoal unfolding KK by auto
+    subgoal by auto
+    subgoal by auto
+    subgoal by (auto simp: additional_WS_invs_def)
+    subgoal by auto
+    subgoal by auto
+    subgoal by auto
+    subgoal unfolding KK by auto
+    subgoal by (auto simp: pending_list_pending)
+    subgoal by fast
+    subgoal by auto
+    subgoal by auto
+    subgoal by auto
+    subgoal by auto
+    subgoal by auto
+    done
+qed
+
+
+lemma cdcl_twl_stgy_prog_list'_spec_final:
+  assumes \<open>twl_struct_invs (twl_st_of S)\<close> and \<open>twl_stgy_invs (twl_st_of S)\<close> and
+    \<open>working_queue_list S = {#}\<close> and
+    \<open>get_conflict_list S = None\<close> and \<open>additional_WS_invs S\<close>
+  shows
+    \<open>cdcl_twl_stgy_prog_list' S \<le> SPEC(\<lambda>T. full cdcl_twl_stgy (twl_st_of S) (twl_st_of T))\<close>
+  apply (rule order_trans[OF cdcl_twl_stgy_prog_list'_spec[THEN refine_pair_to_SPEC,
+          of S \<open>twl_st_of S\<close>]])
+  using assms apply auto[2]
+  apply (rule order_trans)
+   apply (rule ref_two_step[OF _ cdcl_twl_stgy_prog_spec[of \<open>twl_st_of S\<close>],
+        of _ \<open>{(S, S'). S' = twl_st_of S \<and> True}\<close>])
+  using assms by (auto simp: full_def pending_list_pending get_conflict_list_get_conflict
+      pw_conc_inres pw_conc_nofail pw_ords_iff(1))
+
 end
